src/FlatDestCheckComp.v
@@ -402,8 +402,11 @@ Section Preservation.
   Theorem fsim :
     Semantics.forward_simulation (A.semantics prog) (B.semantics tprog).
   Proof.
-    eapply Semantics.forward_simulation_step with (match_states := I').
-    - inversion 1. (* TODO - replace with callstate matching *)
+    eapply Semantics.forward_simulation_step with
+        (match_states := I')
+        (match_values := @eq value).
+    - simpl. intros. eexists. split. 2: econstructor.
+      on >B.is_callstate, invc. repeat i_ctor. all: firstorder discriminate.
     - intros0 II Afinal. invc Afinal. invc II. on >I, invc. on >I_cont, invc. eexists; split. constructor. reflexivity.
     - intros0 Astep. intros0 II.
       eapply I'_sim; try eassumption.
