src/FlatIntTagComp.v
@@ -483,9 +483,13 @@ Section Preservation.
   Theorem fsim :
     Semantics.forward_simulation (A.semantics prog) (B.semantics tprog).
   Proof.
-    eapply Semantics.forward_simulation_step with (match_states := I).
-    - inversion 1. (* TODO - replace with callstate matching *)
-    - intros0 II Afinal. invc Afinal. invc II. on >I_cont, invc. eexists; split. constructor. reflexivity.
+    eapply Semantics.forward_simulation_step with
+        (match_states := I)
+        (match_values := I_value).
+    - simpl. intros. eexists. split. 2: econstructor.
+      on >B.is_callstate, invc. repeat i_ctor.
+    - intros0 II Afinal. invc Afinal. invc II. on >I_cont, invc. eexists; split; eauto.
+      constructor.
     - intros0 Astep. intros0 II.
       eapply I_sim; eauto.
       destruct prog, tprog. eapply compile_cu_I_env; eauto.
